\documentclass[12pt]{article}

% packages
\usepackage{geometry}
\usepackage{amsmath}
\usepackage{amsfonts}

% custom commands
\newcommand{\Q}[1]{\subsubsection*{Problem #1}}

\newcommand{\D}[2]{
\frac{\partial #1}{\partial #2}
}

\newcommand{\opL}{\mathcal{L}}

\newcommand{\dD}[2]{
\frac{\partial^2 #1}{\partial {#2}^2}
}


% parameters
\geometry{hmargin=1cm,vmargin=1cm}
\title{ORF538 - Problem Set 1}
\author{Bachir EL KHADIR }

\begin{document}

\maketitle

\Q{1}

\begin{itemize}

\item
Let $v(t, x) = e^{-t}u(t, x)$, so that 
\begin{align}
\D v t &= e^{-t}(\D u t + u) \\
&= -e^{-t}(\frac12 \dD u x + \D u x) \\
&= -\frac12 \dD v x - \D v x \\
&= -\opL v
\end{align}

and the boundary condition $v(T, x) = e^{-T} u(T, x)= e^{-T - |x|}$

This is a Backward Kolmogorov Equation. The probabilstic representation is thus:

$$v(t, x) = \mathbb{E}_{t,x}\{ e^{-T - |X_T|}\}$$
with $X_t$ a stochastic process of which $\opL$ is the generator. If $(W_s)_s$ a standard brownian motion, we can take $\rm{d} X_s =  \rm{d}s + \rm{d}W_s$, or $X_s = X_t + (t-s) + (W_t - W_s) = x + t-s + (W_t - W_s) \sim \mathcal{N}(x+t-s, (t-s))$


\begin{align*}
u(t, x) &= e^T v(t, x) \\
&= e^T \mathbb{E}_{t,x}\{ e^{-T - |X_T|}\} \\
&= \mathbb{E}_{t,x}\{ e^{-|X_T|}\} \\
&= \mathbb{E}_{t,x}\{ e^{-|X_T|}\} \\
\end{align*}

\item

If $N \sim \mathcal(0, 1)$


\begin{align*}
u(t, x) &= \mathbb{E}_{t,x}\{ e^{-|X_T|}\} \\
&= \mathbb{E}\{ e^{-|x + T - t + \sqrt{T-t} N |}\} \\
&= \mathbb{E}\{ e^{-(a + b N)} 1_{N \geq \frac{-a} b} \} + \mathbb{E}\{ e^{a + b N} 1_{N \leq \frac{-a}b} \} \\
&= e^{-a}\mathbb{E}\{ e^{- b N} 1_{N \geq \frac{-a}b}\} +
e^{a} \mathbb{E}\{ e^{b N} 1_{N \leq \frac{-a}b} \} \\
&= \frac{e^{-a}}{\sqrt{2\pi}} \int_{\frac{-a}b}  e^{-b x-\frac12 x^2} \rm{d}x +
\frac{e^a}{\sqrt{2\pi}} \int^{\frac{-a}b}  e^{b x-\frac12 x^2} \rm{d}x \\
&= \frac{e^{-a+\frac{b^2} 2}}{\sqrt{2\pi}} \int_{\frac{-a}b}  e^{-\frac12 (x+b)^2} 
+ \frac{e^{a+\frac{b^2} 2}}{\sqrt{2\pi}} \int^{\frac{-a}b}  e^{-\frac12 (x-b)^2} \\
&= \frac{e^{-a+\frac{b^2} 2}}{\sqrt{2\pi}} (1-\Phi(\frac{-a}{b}-b))
+ \frac{e^{a+\frac{b^2} 2}}{\sqrt{2\pi}} \Phi(\frac{-a}{b}+b)\\
&= \frac{e^{\frac{b^2} 2}}{\sqrt{2\pi}}
\end{align*}

\end{itemize}


\Q{2}





\end{document}

%%% Local Variables:
%%% mode: latex
%%% TeX-master: t
%%% End:

