\documentclass[12pt]{article}

% packages
\usepackage{geometry}
\usepackage{amsmath}
\usepackage{amsfonts}

% custom commands
\newcommand{\Q}[1]{\subsubsection*{Question #1}}
\newcommand{\Exp}[1]{\mathbb{E}[#1]}
\newcommand{\Var}[1]{Var[#1]}
\newcommand{\Pb}[1]{\mathbb{P}(#1)}
\newcommand{\Fil}{\mathcal{F}}
\newcommand{\FExp}[1]{\mathbb{E}[#1 | \Fil]}
\newcommand{\Gil}{\mathcal{G}}
\newcommand{\GExp}[1]{\mathbb{E}[#1 | \Gil]}

% parameters
\geometry{hmargin=1cm,vmargin=1cm}
\title{ORF526 - Problem Set 2}

\author{Bachir EL KHADIR }

\begin{document}

\maketitle

\Q{1}
\begin{itemize}
\item
  $$\Exp{X} = \Exp{\sum \epsilon_i} = \sum \Exp{\epsilon_i} = n
  \Exp{\epsilon} = np$$
  $$\Var{X} = \Var{\sum \epsilon_i} = \sum \Var{\epsilon_i} = n \Var{\epsilon} = n  \Exp{(X-p)^2} = n [ p(1-p)^2 + (1-p)p^2 ] = np(1-p)$$
\item
  $$\Exp{X} = \sum_{n \geq 1} n e^{-\lambda} \frac{\lambda^n}{n!} = e^{-\lambda} \sum_{n \geq 0}  \frac{\lambda^{n+1}}{n!} = \lambda$$
  $$\Var{X} = \Exp{X^2} -\lambda^2 = \sum_{n \geq 1} n^2 e^{-\lambda} \frac{\lambda^n}{n!} - \lambda^2= e^{-\lambda} \lambda \sum_{n \geq 1} (n+1)  \frac{\lambda^n}{n!} - \lambda^2  = \lambda ( 1 + \lambda) - \lambda^2  = \lambda$$

  $$\sum_n (n+1) \frac{x^n}{n!} = \left(\frac{d}{dx} x \sum_n  \frac{x^n}{n!}\right)_{|x=\lambda} = \left(\frac{d}{dx} x e^x \right)_{|x=\lambda} = e^{\lambda}(1+\lambda)$$
\end{itemize}
\Q{2}
\begin{itemize}
\item 0
\item $\Pb{X = k} = (1-p)^{k-1} p$ geometric
\item $\Exp{X} = \sum_{k \geq 1} k (1-p)^{k-1} p = p  \sum_{k \geq 0} (k+1) (1-p)^k = p \left( \frac{d}{dx} \sum_k x^{k+1} \right)_{|x = 1-p} = p\left( \frac{d}{dx} (\frac{1}{1-x} - 1)  \right)_{|x = 1-p} = p \left(\frac{1}{1 - (1-p)}\right)^2 = \frac{1}{p}$
  $$\Var{X} = \frac{1-p}{p^2}$$
\item $$\Exp{2^X} = \sum 2^n p (1-p)^{n-1} = \frac{p}{1-p} \sum_n (2(1-p))^n =\left\{
    \begin{array}{ll}
      \infty & \text{if} \, p \leq \frac{1}{2} \\
      \frac{p}{(1-p)(2p-1)} & \text{else}
    \end{array}
  \right.
  $$
\end{itemize}

\Q{3}

Let's note $Y = \Exp{X | \Fil}$
\begin{itemize}

\item [(i)]
\begin{itemize}
\item $Y$ takes finite number of values $I := Y(\Omega) = \{x_1, ..., x_r\}$
\item $Y$ is constant on the $A_i$
\item As a consequence, either all element of $A_j$ are equal to $x_i$, or no one is. ie $A_j \cap Y^-1(x_i) = \emptyset$ or $A_j \subset Y^{-1}(x_i)$
\item Since $\Omega = \cap_j A_j$, $Y^{-1}(x_i) = \cap A_j \cup Y^{-1}(x_i) = \cap_{Y(A_j) = \{x_i\}}  A_j$ is measurable
\end{itemize}
\item [(ii)] if $\Fil = \{\emptyset, \Omega\}$, $\Exp{X | \Fil} = \frac{\sum_{\omega_n \in \Omega} X(\omega_n) p_n}{P(\Omega} = \Exp{X}$
\item [(iii)] if $X$ if $\Fil$-measurable, $X$ is constant on the $A_i$, otherwise there exist two elements $w_n, w_m$ such that $X(w_n) \neq X(w_m)$, but then $X^-1( X(w_n) ) \cap A_i$ is an element if $\Fil$ and a strict subset of $A_i$ whose measure is not 0.
for $\omega \in A_m$: $$\Exp{X|\Fil}(\omega) = X(\omega ) \frac{\sum_{\omega_n \in A_m}  p_n}{P(A_m)} = X(\omega)$$
\item [(iv)] This is true because $Y$ is a positive linear combination of the $X(\omega_n) \geq 0$
\item [(v)] 
$$\FExp{X Y + Z} = \FExp{X Y} + \FExp{Z}  \text{ by linearity of } \Exp{}$$
Let $\omega \in A_m$, $X$ is constant on $A_m$, so
$$\FExp{X}(\omega) = X(\omega ) \frac{\sum_{\omega_n \in A_m} Y(w_n) p_n}{P(A_m)} = X(\omega) \FExp{Y}(\omega)$$
\item [(vi)]
$\FExp{X}$ is $\Gil$-measurable (by (i)), we conclude by $(iii)$.
\item [(vii)] Independance of $\Fil$
\item [(viii)] $Y \Fil-$measurable is equivalent to $Y$ being constant on each $A_i$: Let's note $Y(A_i)$ this value. Choosing $Y$ is equivalent to choosing the vector $(Y(A_1), ..., Y(A_M)) \in \mathbb{R}^M$

Minimizating this quantity
$$\Exp{(X-Y)^2} = \sum_{A_i} \sum_{\omega_n \in A_i} (X(\omega_n) - Y(A_i))^2 p_n$$
is therefore equivalent to solving the following minimization program:
\begin{align*}
\text{min}_{a_1, ... a_M \in \mathbb{R}^M }  \sum_{A_i} \sum_{\omega_n \in A_i} (X(\omega_n) - a_i)^2 p_n 
&=  \sum_{A_i} \text{min}_{a_i \in \mathbb{R}} \sum_{\omega_n \in A_i} (X(\omega_n) - a_i)^2 p_n
\\ &= \sum_{A_i} \text{min}_{a_i \in \mathbb{R}} \sum_{\omega_n \in A_i} (X(\omega_n) - a_i)^2 p_n
\\ &= \sum_{A_i} \text{min}_{a_i \in \mathbb{R}} f_i(a_i)
\end{align*}

$f : a_i \mapsto \sum_{\omega_n \in A_i} (X(\omega_n) - a_i)^2 p_n$ is a strictly convex function (as positive sun of convex functions), it has an unique absolute minimum $a_i$ that verifies $f'(a_i) = 2 \sum_{\omega_n \in A_i} (a_i - X(\omega_n))p_n = 0$, ie $a_i = \FExp X (A_i)$
\end{itemize}

\Q{4}
It is clear that $(\Omega, \hat \Fil, \hat \mu)$ is a measure space.\\
Let $D \in \hat \Fil$, and Let $A, B, C \subset \Omega$ such that $A \subset B \in \Fil$ and $C \in \Fil$ such that $D = A \cup C$ and $\mu(B) = 0$. \\
Let's also suppose that $\hat \mu (D) = \mu(C) = 0$.\\
Let $E \subset D$, and let's show that $E \in \hat F$. We can write $E = (E \cap A) \cup (E \cap C) \subset B \cup C = (B\cup C) \cup \emptyset$.

\Q{5}
$$1) \Rightarrow 2)$$
$(E_i)_i$ sequence of increasing sets, as a convention $E_{-1} = \emptyset$

$$\mu ( \cup E_i ) = \mu ( \cup (E_i \setminus  E_{i-1}) ) = \sum_i \mu(E_i \setminus E_{i-1}) = \sum_i \mu(E_i) - \mu(E_{i-1})$$

$$\mu(E_j) = \sum_{ i \leq j} \mu(E_i) - \mu(E_{i-1})$$
so $$\mu ( \cup E_i ) - \mu(E_j) = \sum_i \mu(E_i \setminus E_{i-1}) = \sum_{i > j} \mu(E_i) - \mu(E_{i-1}) \rightarrow 0$$ (as the rest of a convergent series)

$$ 2) \Rightarrow 3)$$
Let $(E_i)_i$ be a sequence of decreasing sets, as a convention, $E_{-1} = \Omega$
\begin{align*}
\mu( \cap E_j ) &= \mu( \Omega \setminus \cup E_j^c) \\
&= \mu(\Omega) - \mu(\cup E_j^c) & \text{by $\sigma$-linearity} \\
&= \mu(\Omega) - \lim \mu(E_j^c) & \text{by coninuity from above} \\
&= \lim \mu(\Omega) -  \mu(E_j^c)  \\
&= \lim \mu(\Omega \setminus E_j^c) & \text{by $\sigma$-linearity} \\
&= \lim \mu(E_j) \\
\end{align*}

$$ 3) \Rightarrow 4)$$

\Q{6}

Let's suppose $1)-3)$
\begin{itemize}

\item $1')$ is trivially verified
\item For $2')$, we have $B \setminus A = B \cap A^c = (B^c \cap A)^c \in \mathcal{D}$ (because $A \subset B \Rightarrow A \cap B^c = \emptyset$)
\item For $3')$, $\cup A_n = \cup A_n \setminus A_{n-1} = \cup (A_n \cap A_{n-1}^c) \in \mathcal{D}$
\end{itemize}

Let's suppose $1')-3')$
\begin{itemize}
\item $1)$ is trivially verified
\item For $3)$, $A^c = \Omega \setminus A \in \mathcal{D}$
\item For $2)$, Let's first show that it is true for a finite number of sets.\\
For two disjoint sets $A_1 \cup A_2 = (A_2^c \setminus A_1)^c \in \mathcal{D} $ by $2')$\\
For $n > 2$ sets $A_1, ... A_n$ pairwise disjoint, we write $\cup  A_i = A_1 \cup \cup_{i>1} A_i$. Since $A_1$ and $\cup_{i>1} A_i$ are disjoint, we can apply the same proof as in the case $n=2$.\\
General case:
$\cup A_n = \cup (\cup_{i \leq n} A_n) \in \mathcal{D}$ by $3')$
\end{itemize}

\end{document}

%%% Local Variables:
%%% mode: latex
%%% TeX-master: t
%%% End:




