#+OPTIONS: toc:nil
#+LATEX_HEADER: \usepackage[margin=0.85in]{geometry}
#+LATEX_HEADER: \newtheorem{theorem}{Theorem}[section]
#+LATEX_HEADER: \newtheorem{lemma}[theorem]{Lemma}
#+LATEX_HEADER: \newtheorem{proof}[theorem]{Proof}


#+TITLE: Polynomial approximation for piece wise constant functions
#+AUTHOR: Bachir El Khadir

* Canonical basis
$$0 = x_0 < x_1 < \ldots < x_n = 1$$

$$u(x) = \sum_{i=0}^n c_i 1_{x+i \le x < x_{i+1}}$$

$$P(x) = \sum_{k=0}^d a_k x^k$$

\begin{align*}
\int_0^1 |P(x) - u(x)|^2 dx
&= \int_0^1 P(x)^2 + 2 \sum_{i=0}^n c_i \int_{x_i}^{x_{i+1}} P(x) + \int_0^1 u(x)^2
\end{align*}

We seek to minimize
$$J(a) := \underbrace{\int_0^1 P(x)^2}_{H(a)} + \underbrace{2 \sum_{i=0}^n c_i \int^{x_i}_{x_{i+1}} P(x)}_{l(a)} + \underbrace{\sum_{i=0}^n c_i^2 (x_{i+1} - x_i)}_{cte}$$


\begin{align*}
l(a) &= 2 \sum_{i=0}^n c_i \int^{x_i}_{x_{i+1}} P(x)
\\&= 2 \sum_{i \le n, k \le d} c_i a_k \frac{x_{i+1}^{k+1} - x_i^{k+1}}{k+1}
\\&= 2 \sum_{k \le d}  a_k \frac1{k+1} \sum_{i \le n} c_i(x_{i+1}^{k+1} - x_i^{k+1})
\\&=  l^Ta & (l_k = \frac2{k} \sum_{i \le n} c_i(x_{i+1}^k - x_i^k))
\end{align*}

\begin{align*}
H(a) &= \int_0^1 P(x)^2 dx
\\&= \sum_{i, j} a_i a_j  \int_0^1 x^{i+j} dx
\\&= \sum_{i, j \in \{0 \ldots d\}} \frac1{i+j} a_i a_j
\\&= a^T H a & (H_{ij} = \frac1{i+j-2}\text{ is a Hilbert matrix})
\end{align*}



$$J(a) = a^THa + l^Ta + cte$$


\begin{align*}
J'(a) = 0
&\implies a = -\frac12H^{-1}l
\end{align*}

\begin{align*}
\min J(a) &= -\frac14 l^T H^{-1} l + cte
\\& \le - \frac1{4\sigma_{\max}} ||l||_2^2 + cte
\\& \le - \frac1{2\sigma_{\max}} \sum_{k=1}^{d+1} \frac1{k^2} \left(\sum_{i \le n} c_i(x_{i+1}^k - x_i^k)\right)^2 + \sum_{i=0}^n c_i^2 (x_{i+1} - x_i)
\\& \le - \frac1{2\pi} \sum_{k=1}^{d+1} \frac1{k^2} \left(\sum_{i \le n} c_i(x_{i+1}^k - x_i^k)\right)^2 + \sum_{i=0}^n c_i^2 (x_{i+1} - x_i)
\end{align*}

* Legendre

  $P = \sum_{i=0}^d a_i P_i$

  $$\int_0^1 P^2 = \sum \frac{a_i^2}{2i+1}$$

  $$\int_{x_i}^{x_{i+1}} P_n(x) dx = (n+\frac12)\left( (P_{n+1}(x_{i+1}) - P_{n+1}(x_i)) - (P_{n-1}(x_{i+1}) - P_{n-1}(x_i)) \right)$$

  $$\int_{x_i}^{x_{i+1}} P_n(x) dx = (n+\frac12)\left( (P_{n+1}(x_{i+1}) - P_{n+1}(x_i)) - (P_{n-1}(x_{i+1}) - P_{n-1}(x_i)) \right)$$







  
  $$\frac1{2n+1} P_n(\frac{x+1}2) = \frac{d}{dx}\left( P_{n+1}(\frac{x+1}2) -  P_{n-1}(\frac{x+1}2)\right)$$

  $$\frac2{2n+1} P_n(\frac{x+1}2) = \left(P_{n+1}'(\frac{x+1}2) -  P_{n-1}'(\frac{x+1}2)\right)$$
  $$ P_n = (n+\frac12) (P_{n+1}' -  P_{n-1}')$$


  
