\documentclass[12pt]{article}

% packages
\usepackage{geometry}
\usepackage{amsmath}
\usepackage{amsfonts}
\usepackage{enumitem}
\usepackage{amsthm}





% custom commands
\newcommand{\Q}[1]{\subsubsection*{Question #1}}
\newcommand{\OB}[1]{\overbrace{#1}^{\in F_n}}
\newtheorem{thm}{Theorem}
\newtheorem{lem}[thm]{Lemma}

% parameters
\geometry{hmargin=1cm,vmargin=1cm}
\title{ORF526 - Problem Set 9}
\author{Bachir EL KHADIR }


\begin{document}

\maketitle

\Q{1}
Because it is predictable we have that $E[M_{n+1}|F_n] = M_{n+1}$, and because it is a martingale $E[M_{n+1}|F_n] = M_n$. Therefore $M_n$ is constant equal to $M_0$.

\Q{2}
Let $M_n = X_0 + \sum_{i=0}^{n-1} X_{i+1} - E[X_{i+1}|F_i]$, $A_n = X_n - M_n = \sum_{i=0}^{n-1}E[X_{i+1}|F_i] - X_i$ and as a convention $A_0 = 0$.

Then

\begin{itemize}
\item $(M_n)$ is an $(F_n)$ martingale because
  \begin{itemize}
  \item It is $(F_n)$-adapted: For all $n$, $M_n$ for $i = 0... n-1$, $X_{i+1}$ and $E[X_{i+1}|F_i]$ are $F_n$ measurable.
  \item $M_{n+1} - M_n = X_{n+1} - E[X_{n+1} | F_n]$, so $$E[M_{n+1}|F_n] - M_n = E[M_{n+1} - M_n | F_n] = E[X_{n+1}|F_n] - E[E[X_{n+1} | F_n]|F_n] = 0$$
  \end{itemize}
\item $(A_n)$ is a non-decreasing predictable process because:
  \begin{itemize}
  \item $(A_n)$ is predictable because for $i < n$, $X_i$ and $E[X_{i+1}|F_i$ are $F_i \subset F_n$ measurable
  \item $(A_n)$ is non-decreasing: $A_{n+1} - A_n = E[X_{n+1}|F_n] - X_n \ge 0$ because $X_n$ is a submartingale.
  \end{itemize}
\end{itemize}
The decomposition is unique, because if there exist an other decomposition $X_n = M'_n + A'_n$ with the same properties then:
$M_n - M'_n = A_n - A'_n$, which a marintgale (as the difference of two martingales), and predictable (as the difference of two predictable processes). By question 1, this sequence is constant equal to $A_0 - A'_0 = 0$

\Q{3}
Let $n, p \in \mathbb{N}$,

By the itereated expectation: $$E[M_{n+i+1}M_{n+i}] = E[E[M_{n+i+1}|F_n]M_{n+i}] = E[M_n^2]$$
So:
$$||M_{n+p} - M_{n}||_2^2 = E[|M_{n+p} - M_n|^2] = E[M_{n+p}^2] + E[M_n^2] - 2 E[M_{n+p}M_n] = E[M_{n+p}^2] - E[M_{n}^2]$$

$M_n^2$ is a submartingale, so $E[M_n^2]$ is non-decreasing, and since it is bounded, it converges and therefore $E[M_{n+p}^2] - E[M_{n}^2] \rightarrow_{n,p} 0$
c/c: $||M_{n+p} - M_{n}||_2 \rightarrow_{n,p} 0$, and $(M_n)$ is a cauchy sequence.

\Q{4}
\begin{enumerate}
\item $M_n$ is $L^p$ bounded and $p > 1$, so $(M_n)$ is uniformly integrable, and therefore: $M_n$


\end{enumerate}

\Q{5}
$B_n = \sum_i B_{i+1} - B_i = \sum_i Y_i$

Let $F_n$ be the filtration generated by $B_n$
\begin{enumerate}
\item $B_n$ is $F_n$ adapted, so is $B_n^2-n$
\item $B_n^2$ is $L_1$, and
  \begin{align*}
    E[B_{n+1}^2-(n+1) | B_n]
    &= E[(B_{n+1} - B_n + B_n)^2 - (n+1)]
    \\&= E[(B_{n+1} - B_n)^2 | B_n] + E[B_n^2|B_n] + 2 E[ (B_{n+1} - B_{n})B_n|F_n] - (n+1)
    \\& = E[ \mathcal N(0,1)^2 ] + B_n^2 - (n+1)
    \\&\text{(because  $B_{n+1}-B_n \sim \mathcal N(0,1)$ and is independent from $B_n$)}
    \\& = B_n^2 - n
  \end{align*}

so $B_n^2 - n$ is a martingale.

\item

  where $Y_i = B_{i+1} - B_i \sim \mathcal N(0,1)$ are iid
  $$E[\exp(\sigma B_n - \frac12 \sigma n^2)] =$$
  \end{enumerate}
\Q{6}
\begin{enumerate}
\item
  \begin{align*}
    a\log(b) \le a log(a) + \frac b e
    &\iff \frac a b \log(\frac b a) \le \frac 1 e
    \\ & \iff \frac{ \log(x) } x \le \frac {\log(e)} e & (x = \frac b a)
    \\ & \iff f(x) \le f(e)
  \end{align*}

  Where $f:x \rightarrow \frac{\log(x)}x$ for $x > 0$,
  $f'(x) = \frac {1 - \log(x)} {x^2} = - \frac { \log(\frac x e)}
  {x^2}$
  is positive when $x \le e$ and negative otherwise, so $f$ has a
  global maximum in $x = e$.


  
\end{enumerate}
\Q{8}
By indepedence of the $X_i$, $E[X_1 | S_n, S_{n+1}...] = E[X_1 | S_n, X_{n+1}, ...] = E[X_1 | S_n]$
By symmetry, $E[X_i|S_n] = E[X_n | S_n]$, and therefore:
$S_n = E[S_n | S_n] = \sum_{i=1}^n E[X_i | S_n] = n E[X_1 | S_n]$,
ie $E[X_1 | S_n, S_{n+1}...] = \frac{S_n}{n}$

\end{document}

