\documentclass[12pt]{article}

% packages
\usepackage{geometry}
\usepackage{amsmath}
\usepackage{amsfonts}

% custom commands
\newcommand{\Q}[1]{\subsubsection*{Question #1}}
\newcommand{\Exp}[1]{\mathbb{E}[#1]}
\newcommand{\Var}[1]{Var[#1]}
\newcommand{\Pb}[1]{\mathbb{P}(#1)}

% parameters
\geometry{hmargin=1cm,vmargin=1cm}
\title{ORF526 - Problem Set 2}

\author{Bachir EL KHADIR }

\begin{document}

\maketitle

\Q{1}
\begin{itemize}
\item
  $$\Exp{X} = \Exp{\sum \epsilon_i} = \sum \Exp{\epsilon_i} = n
  \Exp{\epsilon} = np$$
  $$\Var{X} = \Var{\sum \epsilon_i} = \sum \Var{\epsilon_i} = n \Var{\epsilon} = n  \Exp{(X-p)^2} = n [ p(1-p)^2 + (1-p)p^2 ] = np(1-p)$$
\item
  $$\Exp{X} = \sum_{n \geq 1} n e^{-\lambda} \frac{\lambda^n}{n!} = e^{-\lambda} \sum_{n \geq 0}  \frac{\lambda^{n+1}}{n!} = \lambda$$
  $$\Var{X} = \Exp{X^2} -\lambda^2 = \sum_{n \geq 1} n^2 e^{-\lambda} \frac{\lambda^n}{n!} - \lambda^2= e^{-\lambda} \lambda \sum_{n \geq 1} (n+1)  \frac{\lambda^n}{n!} - \lambda^2  = \lambda ( 1 + \lambda) - \lambda^2  = \lambda$$

  $$\sum_n (n+1) \frac{x^n}{n!} = \left(\frac{d}{dx} x \sum_n  \frac{x^n}{n!}\right)_{|x=\lambda} = \left(\frac{d}{dx} x e^x \right)_{|x=\lambda} = e^{\lambda}(1+\lambda)$$
\end{itemize}
\Q{2}
\begin{itemize}
\item 0
\item $\Pb{X = k} = (1-p)^{k-1} p$ geometric
\item $\Exp{X} = \sum_{k \geq 1} k (1-p)^{k-1} p = p  \sum_{k \geq 0} (k+1) (1-p)^k = p \left( \frac{d}{dx} \sum_k x^{k+1} \right)_{|x = 1-p} = p\left( \frac{d}{dx} (\frac{1}{1-x} - 1)  \right)_{|x = 1-p} = p \left(\frac{1}{1 - (1-p)}\right)^2 = \frac{1}{p}$
  $$\Var{X} = \frac{1-p}{p^2}$$
\item $$\Exp{2^X} = \sum 2^n p (1-p)^{n-1} = \frac{p}{1-p} \sum_n (2(1-p))^n =\left\{
    \begin{array}{ll}
      \infty & \text{if} \, p \leq \frac{1}{2} \\
      \frac{p}{(1-p)(2p-1)} & \text{else}
    \end{array}
  \right.
  $$
\end{itemize}

\end{document}

%%% Local Variables:
%%% mode: latex
%%% TeX-master: t
%%% End:



