% Created 2016-03-30 Wed 21:13
% Intended LaTeX compiler: pdflatex
\documentclass[11pt]{article}
\usepackage[utf8]{inputenc}
\usepackage[T1]{fontenc}
\usepackage{graphicx}
\usepackage{grffile}
\usepackage{longtable}
\usepackage{wrapfig}
\usepackage{rotating}
\usepackage[normalem]{ulem}
\usepackage{amsmath}
\usepackage{textcomp}
\usepackage{amssymb}
\usepackage{capt-of}
\usepackage{hyperref}
\usepackage{minted}
\usepackage[margin=0.5in]{geometry}
\usepackage{amsmath}
\usepackage{amsfonts}
\newcommand{\Problem}[1]{\subsection*{Problem #1}}
\newcommand{\Q}[1]{\subsubsection*{Q.#1}}
\newcommand{\union}[1]{\underset{#1}{\cup} }
\newcommand{\bigunion}[1]{\underset{#1}{\bigcup} \, }
\newcommand{\inter}[1]{\underset{#1}{\cap} }
\newcommand{\biginter}[1]{\underset{#1}{\bigcap} }
\newcommand{\minimize}[3]{\optimize{#1}{#2}{#3}{min}}
\newcommand{\maximize}[3]{\optimize{#1}{#2}{#3}{max}}
\DeclareMathOperator{\cov}{cov}
\DeclareMathOperator{\var}{var}
\author{Bachir El khadir}
\date{\textit{<2016-03-24 Thu>}}
\title{Problem set 6, ORF527}
\hypersetup{
 pdfauthor={Bachir El khadir},
 pdftitle={Problem set 6, ORF527},
 pdfkeywords={},
 pdfsubject={},
 pdfcreator={Emacs 24.5.1 (Org mode )}, 
 pdflang={English}}
\begin{document}

\maketitle

\section{Q1 (8.2 in Steele)}
\label{sec:orgheadline1}

\(f(t, x) = h(t)x \in C^{1,2}(R^+ \times R)\), \(f_t = h'(x), f_x = h(t), f_{xx} = 0\)

So by Ito formula:

$$d(h(t)B_t) = h'(t)B_t dt + h(t)dB_t$$

e.g

$$\int_0^t h(s) dB_s = h(t)B_t - \int_0^t h'(s)B_sds$$

\section{Q2}
\label{sec:orgheadline2}
\textbf{a.}

\(f \in C^{\infty}\), \(f_t = (\mu - \sigma^2/2)f\), \(f_x = \sigma f\), \(f_xx = \sigma^2 f\), By ito formula:

\(dX_t = df(t, W_t) = (f_t + \frac12 f_xx) dt + f_x dW_t = \mu X_t dt + \sigma X_t dW_t\)

\(dX_tdX_t = \sigma^2 X_t^2 dt\)

\(\log' = \frac1x, \log'' = -\frac1{x^2}\), so:

\(d\log(X_t) = \frac{1}{X_t} dX_t - \frac12 \frac1{X_t} \sigma^2 X_t^2 dt = (\mu - \sigma^2/2)dt + \sigma dW_t\)

\textbf{b.}

\(\tau_n = \inf \{ t \ge 0, X_t \le \frac1n \}\)

\(\tau_n\) is non-decreasing, and since \(X_t > 0\), \(\tau_n \rightarrow \infty\) (otherwise \(X_{\tau_n} \rightarrow X_{\lim \tau_n} = 0\))

Let  \(\phi \in C^{\infty}(\mathbb R^+)\) such that:
\[\phi(x) = \begin{array}{cc}
  1 & \text{when } x \ge 1\\
  0 & \text{when } x \le \frac12
  \end{array}
  \]
(The construction has been done in class)

Let \(f^n(t, x) = f(t, x)\phi(nx) \in C^{1, 2}(\mathbb R^+ \times R^+)\). \(f^n\) is equal to \(f\) when \(x \in[\frac1n, \infty)\). 

Then \(\forall t \ge 0\), \(f(t \wedge \tau_n, X_{t \wedge \tau_n}) = f^n(t \wedge \tau_n, X_{t \wedge \tau_n})\)

Let \(n\) be large enough so that \(\frac1n < X_0\). Ito formula applied to \(f^n\):

\(f^n(t, X_t) = f^n(0, X_0) + \int_0^t (f^n_t + \frac{[X]_s}2 f^n_{xx})(s, X_s) ds + \int_0^t (f^n_t + \frac{[X]_s}2 f^n_{xx})(s, X_s) ds\)

So:
\begin{align*}
f(t \wedge \tau_n, X_{t \wedge \tau_n})
&= f^n(t \wedge \tau_n, X_{t \wedge \tau_n})
\\&= f(0, X_0) + \int_0^{t\wedge \tau_n} (f^n_t + \frac{[X]_s}2 f^n_{xx})(s, X_s) ds + \int_0^{t\wedge \tau_n} f^n_{x}(s, X_s) dX_s
\\&= f(0, X_0) + \int_0^{t\wedge \tau_n} (f_t + \frac{[X]_s}2 f_{xx})(s, X_s) ds + \int_0^{t\wedge \tau_n} f_{x}(s, X_s) dX_s
\end{align*}


\(| f(s) - f^n(s)1_{s \le \tau_n}| \le |f(s) - f^n(s)| + |1_{s \le \tau_n} - 1| |f^n(s)| \le |f - f^n|_{\infty} + 2|1_{s \le \tau_n} - 1| |f|_{\infty}\)

As a conclusion

$$f(t, X_t)
  = f(0, X_0) + \int_0^t (f_t + \frac{[X]_s}2 f_{xx})(s, X_s) ds + \int_0^t  f_{x}(s, X_s) dX_s$$


\section{Q3}
\label{sec:orgheadline3}

\textbf{a.}

$$QV[B, t] = \lim_{n \infty} \frac{t}{2^n} \sum_{k=1}^{2^n} |N_k|^2$$

Where \(N_k \overset{iid}{\sim} \mathcal N(0, 1)\) 


By law of large number \(QV[B, t] \rightarrow t E[N_1^2] = t\)


\textbf{b.} 
$$X_t = X_0 + \int_0^t F_s ds + \int_0^t G_s dB_s$$

Using \((b-a)^2 = b^2 - a^2 - 2a(b-a)\)

\begin{align*}
QV[X, T]
&= \lim_{n \infty} \sum_{k=1}^{2^n} (X_{k2^{-n}t} - X_{(k-1)2^{-n}t})^2
\\&= \lim_{n \infty} \sum_{k=1}^{2^n} (X_{k2^{-n}t}^2 - X_{(k-1)2^{-n}t}^2) + \sum_{k=1}^{2^n} 2 X_{(k-1)2^{-n}t}(X_{k2^{-n}t} -  X_{(k-1)2^{-n}t})
\\&= X_t^2 - X_0^2  + 2 \lim_{n \infty} \sum_{k=1}^{2^n} X_{(k-1)2^{-n}t}(X_{k2^{-n}t} -  X_{(k-1)2^{-n}t})
\end{align*}


\begin{align*}
\sum_{k=1}^{2^n} X_{(k-1)2^{-n}t}(X_{k2^{-n}t} -  X_{(k-1)2^{-n}t})
&= \sum_{k=1}^{2^n} X_{(k-1)2^{-n}t} \int_{t_{k-1}}^{t_k} F_s ds + X_{(k-1)2^{-n}t} \int_{t_{k-1}}^{t_k} G_s dB_s
\\&=  \int_0^t \tilde X^n_s F_s ds + \int_0^t  \tilde X^n_s G_s dB_s
\end{align*}

Where \(\tilde X^n_t = \sum_{k=1}^{2^n} X_{t_k} 1_{t_k \le t \le t_{k+1}}\)

\(|\int_0^t \tilde X^n_s F_s ds - \int_0^t \tilde X_s F_s ds| \le \int_0^t |\tilde X^n_s - X_s| |F_s| ds \le \underbrace{\sup_{|u-v| \le 2^{-n}} |X_u - X_v|}_{\rightarrow_n 0 \text{(uniform continuity)}} |F|_{H_1}\)

Let \(\tau_m = \inf\{t , |G_t| \ge m \vee |X_t| \ge m\}\) be a localising sequence. Note that since \(G_t, X_t\) are finite a.s, \(\tau_m \rightarrow \infty\) too.

\begin{align*}
P(|\int_0^t \tilde X_s^nG_sdB_s -  \int_0^t X_sG_sdB_s| > \varepsilon)
&\le P(|\int_0^t \tilde X_s^nG_sdB_s -  \int_0^t X_sG_sdB_s| > \varepsilon, t \le \tau_m) + P(t \ge \tau_m)
\\&\le P(|\int_0^{t \wedge \tau_m} \tilde X_s^nG_sdB_s -  \int_0^{t \wedge \tau_m} X_sG_sdB_s| > \varepsilon) + P(t \ge \tau_m)
\\&\le \frac1{\varepsilon^2}E|\int_0^{t \wedge \tau_m} (\tilde X_s^n - X_s)G_sdB_s |^2 + P(t \ge \tau_m)
&\text{(markov)}
\\&\le \frac{m^2}{\varepsilon^2}\int_0^t E| 1_{t \le \tau_m} (\tilde X_s^n - X_s)^2 |ds + P(t \ge \tau_m)
\\&\le \frac{m^2t}{\varepsilon^2}\int_0^t E 1_{t \le \tau_m} (\tilde X_s^n - X_s)^2 ds + P(t \ge \tau_m)
\end{align*}

By continuity: \(\forall s \; \tilde X_s^n  \rightarrow X_s\), and \(|1_{t \le \tau_m} (\tilde X_s^n - X_s)^2| \le m\), by dominated convergence theorem:

$$\int_0^t E 1_{t \le \tau_m} (\tilde X_s^n - X_s)^2 ds  \rightarrow_n 0$$

so \(\lim\sup_n P(|\int_0^t \tilde X_s^nG_sdB_s -  \int_0^t X_sG_sdB_s| > \varepsilon) \le P(t \ge \tau_m) \rightarrow_m 0\)

We have just proved that
$$QV(X, t) \overset{\mathbb P}{\rightarrow} X_t^2 - X_0^2 - 2\int_0^2 X_s dX_s$$

\textbf{c}

By Ito formula

\(d(X_t^2) = 2X_tdX_t + G_t^2 dt\)

So \(X_t^2 - X_0^2 - \int_0^t X_s dX_s = \int_0^t G_s^2 ds\)

e.g \(QV(X, t) = \int_0^t G_s^2 ds\).

\section{Q4}
\label{sec:orgheadline4}

Let's assume \(X_0 + \int_0^t F_s ds + \sum_{k=1}^m \int_0^t G_s^k
  dW^k_s = \tilde X_0 + \int_0^t \tilde F_s ds + \sum_{k=1}^m \int_0^t
  \tilde G_s^k dW^k_s\)

By setting \(t\) to \(0\), \(X_0 = \tilde X_0\)

By linearity: \(\int_0^t (F_s - \tilde F_s) ds = \sum_{k=1}^m \int_0^t
  (\tilde G_s^k - G_s^k) dW^k_s\),

Taking the quadratic variation of both sides, we find that:

$$0 = \sum_{k=1}^m \int_0^t (\tilde G_s^k - G_s)^2 ds$$ Which proves
\(\forall T \ge t \ge 0 \; \int_0^t ||\tilde G_s - \tilde G_s||^2 ds =
  0\), e.g \(G_s \overset{H^2}{=} \tilde G_s\) and that \(\sum_{k=1}^m
  \int_0^t (\tilde G_s^k - G_s^k) dW^k_s = 0\).

This leads to \(\forall T \ge t \ge 0 \; \int_0^t F_s - \tilde F_s =
  0\), by taking the derivative, \(F_s = \tilde F_s\), therefore
\(\int_0^t |F_t - \tilde F_t| dt = 0\)
\end{document}