
\documentclass{article}
\usepackage[utf8]{inputenc}
\usepackage[english]{babel}
\usepackage{graphicx}
\usepackage{amsfonts}
\usepackage{amsmath}
\usepackage{amsthm}
%\usepackage[a4paper, total={7in, 10in}]{geometry}
\newtheorem{theorem}{Theorem}
\newtheorem{definition}{Definition}
\newtheorem{lemma}[theorem]{Lemma}

\begin{document}
\begin{itemize}
\item $X_0 = 0$
\item $X_t - X_s \sim \mathcal N(0, t-s)$
  \begin{proof}
    fix $t_n \rightarrow t, s_n \rightarrow s$, $t_n, s_n$ are dyadic.
    By construction: $X_{t_n} - X_{x_n} \sim \mathcal N(0, t_n - s_n)$
    $X_{t_n} - X_{x_n} \overset{as}{\rightarrow} X_t - X_s$
    $\mathcal N(0, t_n - s_n) \rightarrow \mathcal N(0, t - s)$
  \end{proof}
\item $X_t - X_s \perp \{ X_r : r \le s \} \forall t \ge s$
  \begin{proof}
    $s = k'2^{-n}, t = k2^{-n}$
    Then $X_t - X_s \perp \sigma \underbrace{\{ X_r, r \le s, r = k2^{-n}\}}_{\mathcal F_n}$
    
    Let $Z \text{ bdd } \sigma\{X_r, r \le s\}$-meas, 
    $Y \text{ bdd } \sigma\{X_t - X_s\}$-meas.

    Let's show $E[YZ] = E[Y]E[Z]$.

    Let $Z^{(n)} \rightarrow Z, Y^{(n)} \rightarrow Y$.
    
    We know that $E[Y^{(n)}Z^{(n)}] = E[Y^{(n)}]E[Z^{(n)}]$
    We conclude by DCT.

    Example of such $Z^{(n)}$:
    $Z^{(n)} = E[Z | \mathcal F_n]$

    Martingal convergence theorem: $Z^{(n)} \rightarrow E[Z | \sigma(\underbrace{\cup_n \mathcal F_n}_{\mathcal F'})]$
    $$\mathcal F' = \sigma \{ X_r : r \le s , r \text{ dyadic } \} \overset{?}{=} \sigma \{ X_r : r \le s \} $$
    \begin{itemize}
    \item $\subseteq$ trivial.
    \item $\supseteq$:It is enough to show that $X_r$ is $\mathcal F'$-measurable.
      This follows by continuity.
    \end{itemize}
    
  \end{proof}
\end{itemize}


\end{document}

  

















